LeanHoG/Tactic/Basic.lean
@@ -1,0 +1,302 @@
+import Lean
+import LeanHoG.Graph
+import LeanHoG.Tactic.SearchDSL
+import LeanHoG.Tactic.Options
+import LeanHoG.Invariant.Hamiltonicity.Basic
+
+import Aesop.Util.Basic
+import Std.Data.List.Basic
+
+namespace LeanHoG
+
+open Lean Widget Elab Command Term Meta Qq Tactic
+
+/-- Express the expression `e` as an exists statement over the type given by `name`.
+    If it is of this form return the arguments, otherwise return `none`.
+-/
+def asExistsOver (e : Expr) (type : Name) : MetaM Expr := do
+  if Expr.isAppOf e ``Exists then
+    let args := Expr.getAppArgs e
+    let xTy := args[0]!
+    let body := args[1]!
+    let p ←  Meta.isDefEq xTy (Expr.const type [])
+    if p == true then
+      let (_, _, conclusion) ← Meta.lambdaMetaTelescope body
+      return conclusion
+    else throwError "exists not over expected type {type}"
+  else
+    throwError "not of the form ∃ x, t"
+
+/-- Decompose `e` as an application `f args` and return `args` -/
+def decomposeAppOf (e : Expr) (f : Name) (normalizeFirst := false) : MetaM (Array Expr) := do
+  let e := if normalizeFirst then ← whnf e else e
+  if Expr.isAppOf e f then
+    let args := Expr.getAppArgs e
+    return args
+  else
+    throwError s!"expr not app of {f}"
+
+def decomposeAnd (e : Expr) : MetaM (Expr × Expr) := do
+  let args ← decomposeAppOf e ``And
+  if h : args.size = 2 then
+    return (args[0]'(by rw [h]; norm_num), args[1]'(by rw [h]; norm_num))
+  else
+    throwError "expr not a conjunction"
+
+partial def decomposeAnds (e : Expr) : MetaM (List Expr) := do
+  try
+    let (e₁, e₂) ← decomposeAnd e
+    let es₁ ← decomposeAnds e₁
+    let es₂ ← decomposeAnds e₂
+    return es₁ ++ es₂
+  catch _ =>
+    return [e]
+
+def decomposeNatLe (e : Expr) : MetaM (Option (Expr × Expr)) := do
+  try
+    let args ← decomposeAppOf e ``Nat.le
+    match args with
+    | #[e₁, e₂] => return some (e₁, e₂)
+    | _ => return none
+  catch _ => return none
+
+def decomposeNatLt (e : Expr) : MetaM (Option (Expr × Expr)) := do
+  try
+    let args ← decomposeAppOf e ``Nat.lt
+    match args with
+    | #[e₁, e₂] => return some (e₁, e₂)
+    | _ => return none
+  catch _ => return none
+
+def decomposeLt (e : Expr) : MetaM (Option (Expr × Expr × Expr)) := do
+  try
+    let args ← decomposeAppOf e ``LT.lt
+    match args with
+    | #[type, _, e₁, e₂] => return some (type, e₁, e₂)
+    | _ => return none
+  catch _ => return none
+
+def decomposeLe (e : Expr) : MetaM (Option (Expr × Expr × Expr)) := do
+  try
+    let args ← decomposeAppOf e ``LE.le
+    match args with
+    | #[type, _, e₁, e₂] => return some (type, e₁, e₂)
+    | _ => return none
+  catch _ => return none
+
+
+def decomposeEq (e : Expr) : MetaM (Option (Expr × Expr × Expr)) := do
+  try
+    let args ← decomposeAppOf e ``Eq
+    match args with
+    | #[type, e₁, e₂] => return some (type, e₁, e₂)
+    | _ => return none
+  catch _ => return none
+
+unsafe def decomposeNat (e : Expr) : MetaM Nat := do
+  let n ← evalExpr' Nat ``Nat e
+  return n
+
+unsafe def decomposeBool (e : Expr) : MetaM Bool := do
+  let b ← evalExpr' Bool ``Bool e
+  return b
+
+def isNatSucc (e : Expr) : MetaM Bool := do
+  try
+    let _ ← decomposeAppOf e ``Nat.succ (normalizeFirst := false)
+    return true
+  catch _ =>
+    return false
+
+/-- Returns (type, comparison, lhs rhs) of a comparison. -/
+def decomposeComp (e : Expr) : MetaM (Expr × Expr × Expr × Expr) := do
+  match (← decomposeNatLe e),
+        (← decomposeNatLt e),
+        (← decomposeLt e),
+        (← decomposeLe e),
+        (← decomposeEq e) with
+  | some (lhs, rhs), none, none, none, none => return (mkConst ``Nat, mkConst ``Nat.le, lhs, rhs)
+  | none, some (lhs, rhs), none, none, none => return (mkConst ``Nat, mkConst ``Nat.le, lhs, rhs)
+  | none, none, some (t, lhs, rhs), none, none => return (t, mkConst ``LT.lt, lhs, rhs)
+  | none, none, none, some (t, lhs, rhs), none => return (t, mkConst ``LE.le, lhs, rhs)
+  | none, none, none, none, some (t, lhs, rhs) => return (t, mkConst ``Eq, lhs, rhs)
+  | _,_,_,_,_ => throwError "expr {e} not a comparison"
+
+def asBoolInvariant (e : Expr) : MetaM BoolInvariant := do
+  match e with
+  | .const f _  =>
+    match f with
+    | ``Graph.isTraceable => return .Traceable
+    | ``Graph.isHamiltonian => return .Hamiltonian
+    | n => throwError s!"not known invariant: {n}"
+  | _ => throwError "expr {e} not an invariant"
+
+def asInvariant (e : Expr) : MetaM Invariant := do
+  match e with
+  | .const f _  =>
+    match f with
+    -- | ``Graph.isTraceable => return (.BoolInvariant .Traceable)
+    -- | ``Graph.isHamiltonian => return (.BoolInvariant .Hamiltonian)
+    | ``Graph.vertexSize =>  return (.IntegralInvariant .NumberOfVertices)
+    | ``Graph.edgeSize => return (.IntegralInvariant .NumberOfEdges)
+    | n => throwError s!"not known invariant: {n}"
+  | _ => throwError "expr {e} not an invariant"
+
+/-- Missing NEGATION case -/
+def decomposeProp (e : Expr) : MetaM (BoolInvariant × Bool) := do
+  match e with
+  | .app f args =>
+    -- Have to check if application of negation
+    try
+      let _ ← decomposeAppOf e ``Not
+      let (inv, _) ← decomposeProp args
+      return (inv, false)
+    catch _ =>
+      let inv ← asBoolInvariant f
+      return (inv, true)
+  | _ =>
+    throwError s!"unknown prop {e}"
+
+def decomposeInvariantApp (e : Expr) : MetaM (Option (Invariant × Expr)) := do
+  match e with
+  | .app f args =>
+    try
+      let inv ← asInvariant f
+      return some (inv, args)
+    catch _ => return none
+  | _ => return none
+
+def asComparisonOp (e : Expr) : MetaM ComparisonOp := do
+  match e with
+  | .const f _  =>
+    match f with
+    | ``Eq => return .Eq
+    | ``Nat.lt => return .Lt
+    | ``Nat.le => return .Le
+    | ``LE.le => return .Le
+    | ``LT.lt => return .Lt
+    | _ => throwError s!"expr {e} not a comparison"
+  | _ => throwError s!"expr {e} not a comparison"
+
+unsafe def decomposeComparison (type op lhs rhs : Expr) :
+  dbg_trace s!"{lhs}, {rhs}"
+  MetaM HoGEnquiry := do
+  if ← (isDefEq type (mkConst ``Nat)) then
+    match (← decomposeInvariantApp lhs), (← decomposeInvariantApp rhs) with
+    | some (.IntegralInvariant ii, _args), none =>
+      let n ← decomposeNat rhs
+      let op ← asComparisonOp op
+      return .IntegralEnquiry { inv := ii, op := op, val := n }
+    | none, some (.IntegralInvariant ii, _args) =>
+      let n ← decomposeNat rhs
+      let op ← asComparisonOp op
+      return .IntegralEnquiry { inv := ii, op := op, val := n }
+    | _, _ => throwError "comparison not of expected form"
+  else if ← (isDefEq type (mkSort levelZero)) then
+    match (← decomposeInvariantApp lhs), (← decomposeInvariantApp rhs) with
+    | some (.BoolInvariant bi, _), none =>
+      let b ← decomposeBool rhs
+      let _op ← asComparisonOp op -- TODO: Check the comparison is equality
+      return .BoolEnquiry { inv := bi, val := b }
+    | none, some (.BoolInvariant bi, _) =>
+      let b ← decomposeBool rhs
+      let _op ← asComparisonOp op -- TODO: Check the comparison is equality
+      return .BoolEnquiry { inv := bi, val := b }
+    | _, _ => throwError "comparison not of expected form"
+  else
+    throwError "comparison not of expected form"
+
+unsafe def decompose (e : Expr) : MetaM (List HoGEnquiry) := do
+  let body ← asExistsOver e ``Graph
+  let args ← decomposeAnds body
+  let comparisons ← args.mapM (fun (arg : Expr) => do
+    try
+      let (t,op,lhs,rhs) ← decomposeComp arg
+      let enq ← decomposeComparison t op lhs rhs
+      return enq
+    catch _ =>
+      let (inv, val) ← decomposeProp arg
+      return .BoolEnquiry { inv := inv, val := val }
+  )
+  return comparisons
+
+def buildEnquiry (e : Expr) : MetaM (Option HoGEnquiry) := do
+  sorry
+
+def buildQuery (e : Expr) : MetaM (Option (List HoGEnquiry)) := do
+  sorry
+
+syntax (name := searchForExampleInHoG) "search_for_example" : tactic
+
+instance : ToString (Invariant × ComparisonOp × Nat) where
+  toString := fun (i, op, n) =>
+    s!"{i} {op} {n}"
+
+#check Declaration
+
+@[tactic searchForExampleInHoG]
+unsafe def searchForExampleInHoGImpl : Tactic
+  | stx@`(tactic|search_for_example) =>
+    withMainContext do
+      let goal ← getMainGoal
+      let goalDecl ← goal.getDecl
+      let goalType := goalDecl.type
+      let graphType : Expr ← mkConst ``Graph
+      let exists_intro ← mkConst ``Exists.intro
+      try
+        let enqs ← decompose goalType
+        let hash := hash enqs
+        -- IO.println s!"{hash}"
+        let query := HoGQuery.build enqs
+        let graphs ← liftCommandElabM (queryDatabaseForExamples [query] hash)
+        if h : graphs.length > 0 then
+          let ⟨graphId⟩ := graphs[0]'(by simp_all only [not_lt_zero'])
+          -- IO.println f!"Found such a graph: {name}"
+          let mvarIds' ← Lean.MVarId.apply goal exists_intro
+          replaceMainGoal mvarIds'
+          let newGoals ← getGoals
+          for goal in newGoals do
+            -- find the goal with type Graph and try to close it with `graph`
+            let goalDecl ← goal.getDecl
+            let goalType := goalDecl.type
+            if ← Meta.isDefEq goalType graphType then
+              -- check that the goal is not already assigned
+              goal.checkNotAssigned `search_for_counterexample
+              -- try to close the goal with the found graph
+              goal.withContext do
+                let r ← Lean.Elab.Tactic.elabTermEnsuringType graphId goalType
+                goal.assign r
+              -- Now try to simp which will among other things look for instance for e.g. HamiltonianPath
+              evalSimp stx
+              Lean.logInfo s!"Closed goal using {graphId.getId}"
+            else
+              continue
+        else
+          throwError "Could not find any graphs matching criteria"
+
+      catch e =>
+        throwError m!"search failed: {e.toMessageData}"
+
+  | _ => throwUnsupportedSyntax
+
+-- #search_hog hog{ numberOfVertices < 5 ∧ traceable = true }
+
+set_option leanHoG.pythonExecutable "/home/jure/source-control/Lean/Lean-HoG/.venv/bin/python"
+
+def a : Nat := 2
+
+elab "use_a" : tactic =>
+  Lean.Elab.Tactic.withMainContext do
+    let goal ← Lean.Elab.Tactic.getMainGoal
+    closeMainGoalUsing (checkUnassigned := false) fun type => do
+      let a_name := mkIdent ``a
+      let r ← Lean.Elab.Tactic.elabTermEnsuringType a_name type
+      return r
+
+example : Nat := by
+  exact a
+
+example : ∃ (G : Graph), G.vertexSize = 7 ∧ G.isTraceable := by
+  search_for_example
+
+end LeanHoG
